\documentclass[10pt]{article}
\usepackage{amsmath}
\input{style}
\title{Solution of assignment \#1}
\begin{document}
\maketitle
\begin{enumerate}
\item Using $\tilde{\omega}^a.\boldsymbol{e}_b = \delta^a_b$, $\boldsymbol{e}_a.\boldsymbol{e}_b = g_{ab}$ and $\tilde{\omega}^a.\tilde{\omega}^b = g^{ab}$, prove that $g^{ab}$ is the inverse of $g_{ab}$.
  \begin{align}
    \label{eq:1}
    g_{ab}g^{bc}
    & = (\boldsymbol{e}_a . \boldsymbol{e}_b) (\tilde{\omega}^b . \tilde{\omega}^c)\\
    & = (\boldsymbol{e_a}.\tilde{\omega}^c) (\boldsymbol{e}_b . \tilde{\omega}^b)\\
    & = \delta^c_a
  \end{align}
\item Using the coordinate transformations $\boldsymbol{e}_{a'} = \boldsymbol{e}_{a}M^a_{a'}$, $\tilde{\omega}^{a'} = M^{a'}_{a}\tilde{\omega}^a$ and the inverse matrices $M^{a'}_b = (M^b_{a'})^{-1}$, prove that the components of the vectors, $\boldsymbol{A} = A^ae_a$, dual-vectors, $\tilde{\boldsymbol{B}} = B_b \tilde{\omega}^b$, and mixed tensors, $\boldsymbol{T} = T^a_b e_a \tilde{\omega}^b$, are transformed as $A^{a'} = M^{a'}_a A^a$, $B_{a'} = B_a M^{a}_{a'}$ and $T^{a'}_{b'} = M^{a'}_a T^a_b M^{b}_{b'}$, respectively.

  \begin{align}
    \label{eq:2}
    \boldsymbol{A}
    & = A^{a}e_{a}\\
    & = A^{a}e_{a'} M^{a'}_{a}\\
    & = A^{a}M^{a'}_{a}e_{a'}\\
    & = A^{a'} e_{a'}
  \end{align}
  implies $A^{a'} = A^{a}M^{a'}_{a}$

  \begin{align}
    \label{eq:3}
    \boldsymbol{\tilde{B}}
    & = B_b\tilde{\omega}^b\\
    & = B_b \tilde{\omega}^{b'} M^{b}_{b'}\\
    & = B_b M^{b}_{b'}\tilde{\omega}^{b'}\\
    & = B_{b'}\tilde{\omega}^{b'}
  \end{align}
  implies $B_{a'} = B_{a} M^{a}_{a'}$.
  Finally,
  \begin{align}
    \label{eq:4}
    \boldsymbol{T}
    & = T^{a}_b e_a \tilde{\omega}^b\\
    & = T^{a}_b e_{a'}M^{a'}_{a}\tilde{\omega}^{b'}M^{b}_{b'}\\
    & = T^{a}_{b}M^{a'}_{a}M^{b}_{b'}e_{a'}\tilde{\omega}^{b'}\\
    & = T^{a'}_{b'}e_{a'}\tilde{\omega}^{b'}
  \end{align}
  implying $T^{a'}_{b'} = T^{a}_{b} M^{a'}_{a}M^{b}_{b'}$.
  
\item Using the Bianchi identities,
  \begin{equation}
    \label{eq:bianchi-identities}
    \nabla_e\R{abcd} + \nabla_d\R{abec} + \nabla_c\R{abde} = 0,
  \end{equation}
  prove that $\nabla^aG_{ab} = 0$, where
  \begin{equation}
    \label{eq:Gab}
    G_{ab} = \R{ab} - \frac{1}{2}g_{ab} \R{}
  \end{equation}

  We start by contracting Eq. \eqref{eq:bianchi-identities} with $g^{ac}$ which gives
  \begin{equation}
    \label{eq:3-1}
    \nabla_{e}\R{bd} - \nabla_d \R{be} + \nabla^a\R{abde} = 0
  \end{equation}
  where we have used $\R{abcd} = - \R{abdc}$ in the second term. Now we contract Eq. \eqref{eq:3-1} with $g^{eb}$ to get
  \begin{equation}
    \label{eq:}
    2 \nabla^b \R{bd} - \nabla_d \R{} = 0 \Rightarrow \nabla^a\R{ab} - \frac{1}{2} \nabla^a (g_{ab}\R{}) = 0 \Rightarrow \nabla^a G_{ab} = 0
  \end{equation}

\item Derive the curvature invariants $R^{ab}R_{ab}$ and $R$ for Schwarzschild and Kerr spacetime in the vacuum case.

  Einstein's Field equation is given by
  \begin{equation}
    \label{eq:EFE}
    R_{ab} + \frac{1}{2} g_{ab}R = 0
  \end{equation}
  contracting with $g^{ab}$ gives
  \begin{equation}
    \label{eq:}
    g^{ab}R_{ab} + \frac{1}{2} g^{ab}g_{ab}R = 0 \Rightarrow R + R = 0 \Rightarrow R = 0
  \end{equation}
  From which it automatically follows that $R^{ab}R_{ab} = 0$.

\item Exercise 2.1 of Baumgarte and Shapiro.
\item Exercise 2.12-2.14 of Baumgarte and Shapiro.
  \begin{enumerate}
  \item The acceleration is given by
    \begin{equation}
      \label{eq:acceleration}
      a_a = n^b \nabla_b n_a
    \end{equation}
    Component along $n^a$ is given by
    \begin{equation}
      \label{eq:projection-along-na}
      n^aa_a = n^a n^b \nabla_b n_a = \frac{1}{2}  n^b \nabla_b(n^an_a) = 0
    \end{equation}

  \item 
  \item \begin{equation}
      \label{eq:alpha}
      \alpha = \frac{1-M/(2r)}{1+M/(2r)},\qquad n^a = (1/\alpha, 0, 0, 0)
    \end{equation}
    \begin{align}
      \label{eq:acceleration}
      a_a
      & = D_a \ln \alpha\\
      & = (n^b n_a + \delta^b_a)\nabla_b \ln \alpha\\
      & = n^b n_a \partial_b\ln\alpha + \partial_a\ln \alpha\\
      & = n_a (1/\alpha)\partial_t\ln\alpha + \partial_r \ln\alpha \delta^r_a\\
      & = 0 + \delta^r_a \frac{4Mr^2}{r^2 - M^2}\\
      & = \delta^r_a \frac{4Mr^2}{r^2 - M^2}
    \end{align}
  \end{enumerate}
  
\item Exercise 2.34 of Baumgarte and Shapiro.\\
  \begin{enumerate}
  \item Comparing the Kerr metric with Eq. 2.119 and 2.122 
    \begin{equation}
      \label{eq:metric-in-alpha-beta}
      -\alpha^{-2} = g^{tt} \Rightarrow \alpha = \sqrt{-1/g^{tt}} = \sqrt{\frac{\left(a^2+r (r-2 M)\right) \left(a^2 \cos (2 \theta )+a^2+2 r^2\right)}{a^4+a^2 \cos (2 \theta ) \left(a^2+r (r-2 M)\right)+a^2 r (2 M+3 r)+2 r^4}},
    \end{equation}
    \begin{equation}
      \label{eq:beta}
      \beta_i = \delta_{\phi i} g_{t\phi} = -\frac{2 a M r \sin ^2(\theta )}{a^2 \cos ^2(\theta )+r^2}\delta_{i\phi}
    \end{equation}
    and
    \begin{equation}
      \label{eq:gamma}
      \gamma_{ij} = \delta_{ij}g_{ij}
    \end{equation}
    $t^a = (1, 0, 0, 0) = \delta^a_t$ and hence
    \begin{align}
      \label{eq:tnorm}
      t_at^a = g_{ab}t^at^b = g_{tt} = \frac{a^2 \sin ^2(\theta )-a^2+2 M r-r^2}{a^2 \cos ^2(\theta )+r^2}
    \end{align}
    So, $t_at^a$ is negative outside ergsosphere and positive inside the ergsosphere.
  \item Evolution equation of the spatial metric is given by
    \begin{equation}
      \label{eq:evolution-of-spatial-metric}
      \partial_t\gamma_{ij} = -2\alpha K_{ij} + D_i\beta_j + D_j\beta_i.
    \end{equation}
    As the spatial metric is time independent, the above equation gives (with equation from Ex. 2.30)
    \begin{equation}
      \label{eq:extrinsic-metric}
      K_{ij} = \frac{1}{2\alpha}(\nabla_i\beta_j + \nabla_j\beta_i) = \frac{1}{2\alpha}(\partial_i\beta_j + \partial_j\beta_i - 2 \Gamma_{ij}^k \beta_k) = \frac{1}{2\alpha}(\partial_ig_{t\phi}\delta_{j\phi} + \partial_jg_{t\phi}\delta_{i\phi} - 2\Gamma_{ij}^\phi g_{t\phi}) ,
    \end{equation}
    and
    \begin{equation}
      \label{eq:christofell}
      \Gamma^\phi_{rr} = \Gamma^\phi_{r\theta} = \Gamma^\phi_{\theta\theta} = \Gamma^\phi_{\phi\phi} = 0
    \end{equation}
    hence,
    \begin{equation}
      \label{eq:krtheta}
      K_{rr} = 0, K_{r\theta} = 0, K_{r\phi} = \frac{1}{2\alpha}(\partial_rg_{t\phi} - 2\Gamma^\phi_{r\phi}), K_{\theta\theta} = 0, K_{\theta\phi} = \frac{1}{2\alpha}(\partial_\theta g_{t\phi}-2\Gamma^\phi_{\theta\phi}), K_{\phi\phi} = 0 
    \end{equation}
    In the limit $r\gg M$ and $r\gg a$, $\alpha \to 1$.
    \begin{equation}
      \label{eq:krphi}
      K_{r\phi} = -\frac{1}{2\alpha}\frac{4 a M \sin ^2(\theta ) \left(a^4+a^2 \left(a^2-r^2\right) \cos (2 \theta )-3 a^2 r^2-6 r^4\right) \left(a^2 \cos (2 \theta )+a^2+2 r (r-2 M)\right)}{\left(a^2+r
   (r-2 M)\right) \left(a^2 \cos (2 \theta )+a^2+2 r^2\right)^3}
\end{equation}
therefore becomes,
\begin{equation}
  \label{eq:krphi2}
  K_{r\phi} = \frac{1}{2}\frac{6aM\sin^2\theta}{r^2} = \frac{3aM\sin^2\theta}{r^2}  
\end{equation}
Similarly,
\begin{equation}
  \label{eq:kthetaphi}
  K_{\theta \phi} = - \frac{1}{2\alpha}\frac{16 a^3 M r \sin ^3(\theta ) \cos (\theta ) \left(a^2 \cos (2 \theta )+a^2+2 r (r-2 M)\right)}{\left(a^2 \cos (2 \theta )+a^2+2 r^2\right)^3} 
\end{equation}
  \end{enumerate}
\end{enumerate}
\end{document}
